(big) use machine ints, extraction, test script

GPU.h
@@ -1,0 +1,6 @@
+#ifndef __PULSE__GPU_H
+#define __PULSE__GPU_H 1
+
+#define PULSE_KCALL(foo, nblk, nthr, ...) foo<<<nblk,nthr>>>(__VA_ARGS__)
+
+#endif
