src/examples/GPU.DotProduct.fst
@@ -5,66 +5,86 @@ open Pulse.Lib.Array
 open Pulse.Lib.Pervasives
 module A = Pulse.Lib.Array
 module SZ = FStar.SizeT
+module U32 = FStar.UInt32
 open Pulse.Lib.BigStar
 open GPU
 
-let size : nat = 1024
+let m_size : SZ.t = 1024sz
+let size : n:(erased nat){reveal n == SZ.v m_size} = SZ.v m_size
 
-let kpre (ga1 ga2 r : gpu_array int size) (nth : nat) (tid:nat{tid < nth}) : slprop =
+let elem_t = U32.t
+
+(* This sucks, clean it up. Multiparam TC? *)
+[@@coercion]
+let uint32_to_int (x:U32.t) : GTot nat = U32.v x
+[@@coercion]
+let uint32_to_erased_nat (x:U32.t) : erased nat = U32.v x
+
+[@@coercion]
+let sizet_to_int (x:SZ.t) : GTot int = SZ.v x
+[@@coercion]
+let sizet_to_erased_nat (x:SZ.t) : erased nat = SZ.v x
+
+[@@coercion]
+inline_for_extraction
+let uint32_to_sizet x = FStar.SizeT.uint32_to_sizet x
+
+let kpre (ga1 ga2 r : gpu_array elem_t (SZ.v m_size)) (nthr : nat) (tid:nat{tid < nthr}) : slprop =
   gpu_pts_to_array1 ga1 tid **
   gpu_pts_to_array1 ga2 tid **
   gpu_pts_to_array1 r tid
 
-let kpost (ga1 ga2 r : gpu_array int size) (nth : nat) (tid:nat{tid < nth}) : slprop =
+let kpost (ga1 ga2 r : gpu_array elem_t (SZ.v m_size)) (nthr : nat) (tid:nat{tid < nthr}) : slprop =
   gpu_pts_to_array1 ga1 tid **
   gpu_pts_to_array1 ga2 tid **
   gpu_pts_to_array1 r tid
 
+[@@CPrologue "__global__"]
 ```pulse
 fn kernel
-  (ga1 ga2 : gpu_array int size)
-  (r : gpu_array int size)
-  (nth : erased nat)
-  (tid : nat{tid < nth})
-  requires gpu ** kpre  ga1 ga2 r nth tid
-  ensures  gpu ** kpost ga1 ga2 r nth tid
+  (ga1 ga2 : gpu_array elem_t size)
+  (r : gpu_array elem_t size)
+  (nthr : erased nat)
+  (etid : erased nat{etid < nthr})
+  requires gpu ** thread_id etid ** kpre ga1 ga2 r nthr etid
+  ensures  gpu ** thread_id etid ** kpost ga1 ga2 r nthr etid
 {
+  let tid = block_idx_x ();
   (* r[tid] = ga1[tid] * ga2[tid] *)
-  
 
-  (**)unfold (kpre ga1 ga2 r nth tid);
+  (**)unfold (kpre ga1 ga2 r nthr tid);
 
   (**)unfold (gpu_pts_to_array1 ga1 tid);
   (**)gpu_pts_to_slice_ref ga1 tid (tid+1); // recall tid < size
-  let v1 = gpu_array_read #int #size #tid #(tid+1) ga1 tid;
+  let v1 = gpu_array_read_u32 #size #tid #(tid+1) ga1 tid;
 
   (**)unfold (gpu_pts_to_array1 ga2 tid);
-  let v2 = gpu_array_read #int #size #tid #(tid+1) ga2 tid;
+  let v2 = gpu_array_read_u32 #size #tid #(tid+1) ga2 tid;
   
-  let v = v1 * v2;
+  let v = v1 `U32.mul_underspec` v2;
   
   (**)unfold (gpu_pts_to_array1 r tid);
-  gpu_array_write #int #size #tid #(tid+1) r tid v;
+  gpu_array_write_u32 #size #tid #(tid+1) r tid v;
 
   (**)fold (gpu_pts_to_array1 r tid);
   (**)fold (gpu_pts_to_array1 ga1 tid);
   (**)fold (gpu_pts_to_array1 ga2 tid);
-  (**)fold (kpost ga1 ga2 r nth tid);
+  (**)fold (kpost ga1 ga2 r nthr tid);
 }
 ```
 
 ```pulse
 fn main (_:unit)
-  requires cpu
+  requires cpu ** pure SizeT.fits_u32
   ensures  cpu
 {
-  let a1 = A.alloc 0 (SZ.uint_to_t size);
-  let a2 = A.alloc 0 (SZ.uint_to_t size);
-  let ar = A.alloc 0 (SZ.uint_to_t size);
+  let a1 = A.alloc #elem_t 0ul m_size;
+  let a2 = A.alloc #elem_t 0ul m_size;
+  let ar = A.alloc #elem_t 0ul m_size;
 
   let mut i = 0sz;
 
-  while (let v = !i; (SZ.v v < size))
+  while (let v = !i; (v `SZ.op_Less_Hat` m_size))
      invariant b.
        exists* v. pts_to i v **
        (exists* s. A.pts_to a1 s ** pure (Seq.length s == size)) **
@@ -72,19 +92,21 @@ fn main (_:unit)
        pure (b == (SZ.v v < size))
   {
     let v = !i;
-    a1.(v) <- SZ.v v;
-    a2.(v) <- SZ.v v;
+    a1.(v) <- FStar.SizeT.sizet_to_uint32 v;
+    a2.(v) <- FStar.SizeT.sizet_to_uint32 v;
     i := SZ.add v 1sz;
     ()
   };
 
-  let ga1 = gpu_array_alloc #int size;
-  let ga2 = gpu_array_alloc #int size;
+  let ga1 = gpu_array_alloc_u32 m_size;
+  let ga2 = gpu_array_alloc_u32 m_size;
 
-  GPU.Array.gpu_memcpy_host_to_device a1 ga1;
-  GPU.Array.gpu_memcpy_host_to_device a2 ga2;
+  GPU.Array.gpu_memcpy_host_to_device_u32 a1 ga1;
+  GPU.Array.gpu_memcpy_host_to_device_u32 a2 ga2;
   
-  let gr = gpu_array_alloc #int size;
+  let gr = gpu_array_alloc_u32 m_size;
+  
+  let nthr : U32.t = SZ.sizet_to_uint32 m_size <: U32.t;
   
   // Slicing the arrays
   (**)gpu_array_slice_1_underspec ga1;
@@ -92,46 +114,57 @@ fn main (_:unit)
   (**)gpu_array_slice_1_underspec gr;
 
   // Boring combination of resources
-  (**)bigstar_zip 0 size (gpu_pts_to_array1 ga1) (gpu_pts_to_array1 ga2);
-  (**)bigstar_zip 0 size _ (gpu_pts_to_array1 gr);
+  (**)bigstar_zip 0 (SZ.v m_size) (gpu_pts_to_array1 ga1) (gpu_pts_to_array1 ga2);
+  (**)bigstar_zip 0 (SZ.v m_size) _ (gpu_pts_to_array1 gr);
 
   (**)rewrite
-    (bigstar 0 size
+    (bigstar 0 (SZ.v m_size)
       (fun i -> (gpu_pts_to_array1 ga1 i **
                  gpu_pts_to_array1 ga2 i) **
                  gpu_pts_to_array1 gr i))
   as
-    (bigstar 0 size (fun i -> kpre ga1 ga2 gr size i));
+    (bigstar 0 (SZ.v m_size) (fun i -> kpre ga1 ga2 gr nthr i));
 
   (**)bigstar_uneta ();
-  
-  launch_kernel_n size (kernel ga1 ga2 gr size);
+
+  assert (pure (SZ.v m_size == U32.v nthr));
+  rewrite
+    (bigstar 0 (SZ.v m_size) (kpre ga1 ga2 gr nthr))
+  as
+    (bigstar 0 (U32.v nthr)  (kpre ga1 ga2 gr nthr));
+
+  launch_kernel_n #0 nthr (fun tid -> kernel ga1 ga2 gr (hide (U32.v nthr)) tid);
+
+  rewrite
+    (bigstar 0 (U32.v nthr)  (kpost ga1 ga2 gr nthr))
+  as
+    (bigstar 0 (SZ.v m_size) (kpost ga1 ga2 gr nthr));
 
   (**)bigstar_eta ();
 
   rewrite
-    (bigstar 0 size (fun i -> kpre ga1 ga2 gr size i))
+    (bigstar 0 (SZ.v m_size) (fun i -> kpre ga1 ga2 gr nthr i))
   as
-    (bigstar 0 size
+    (bigstar 0 (SZ.v m_size)
       (fun i -> gpu_pts_to_array1 ga1 i **
                 gpu_pts_to_array1 ga2 i **
                 gpu_pts_to_array1 gr i));
-  (**)bigstar_unzip 0 size _ _;
-  (**)bigstar_unzip 0 size _ _;
+  (**)bigstar_unzip 0 (SZ.v m_size) _ _;
+  (**)bigstar_unzip 0 (SZ.v m_size) _ _;
   
   // Unslicing
   (**)gpu_array_unslice_1_underspec ga1;
   (**)gpu_array_unslice_1_underspec ga2;
   (**)gpu_array_unslice_1_underspec gr;
   
-  GPU.Array.gpu_memcpy_device_to_host ar gr;
-  gpu_array_free ga1;
-  gpu_array_free ga2;
-  gpu_array_free gr;
+  GPU.Array.gpu_memcpy_device_to_host_u32 ar gr;
+  gpu_array_free_u32 ga1;
+  gpu_array_free_u32 ga2;
+  gpu_array_free_u32 gr;
 
   i := 0sz;
-  let mut psum = 0;
-  while (let v = !i; (SZ.v v < size))
+  let mut psum = 0ul;
+  while (let v = !i; (v `SZ.op_Less_Hat` m_size))
      invariant b. exists* vi vpsum.
        pts_to i vi **
        pts_to psum vpsum  **
@@ -141,7 +174,7 @@ fn main (_:unit)
     let vi = !i;
     let ri = ar.(vi);
     let vpsum = !psum;
-    psum := vpsum + ri;
+    psum := vpsum `U32.add_underspec` ri;
     i := SZ.add vi 1sz;
   };
   
