src/lib/GPU.Base.fsti
@@ -4,6 +4,7 @@ open Pulse.Lib.Pervasives
 open FStar.Tactics.V2
 open FStar.Seq
 open Pulse.Lib.BigStar
+module U32 = FStar.UInt32
 
 (* Token for being in CPU code *)
 val cpu : slprop
@@ -11,32 +12,44 @@ val cpu : slprop
 (* Token for being in GPU code *)
 val gpu : slprop
 
-(*
-  __device__
-  void f() {
-    ...
-  }
+let tid_t = nat
 
-  f<<<1, 1>>>();
-*)
-val launch_kernel_1
+(* Token for being a particular thread *)
+val thread_id : tid_t -> slprop
+
+```pulse
+val
+fn block_idx_x () (#n:erased tid_t)
+  requires thread_id n
+  returns  id : U32.t
+  ensures  thread_id n ** pure (n == U32.v id)
+``` 
+
+(* f<<<1, 1>>>(...); *)
+```pulse
+val
+fn launch_kernel_1
   (#pre #post : slprop)
   (k : unit ->
     stt unit (gpu ** pre) (fun _ -> gpu ** post)
   )
-  : stt unit (cpu ** pre) (fun _ -> cpu ** post)
+  requires cpu ** pre
+  ensures  cpu ** post
+```
 
-(*
-  f<<<n, 1>>>();
-*)
-val launch_kernel_n
+(* f<<<n, 1>>>(...); *)
+```pulse
+val
+fn launch_kernel_n
   (#u1: int)
-  (nthr  : pos)
-  (#pre  : (tid:nat{tid < nthr} -> slprop))
-  (#post : (tid:nat{tid < nthr} -> slprop))
-  (f :
-    (tid:nat{tid < nthr}) ->
-    stt unit (gpu ** pre tid) (fun _ -> gpu ** post tid)
+  (nthr  : U32.t)
+  (#pre  : (tid:nat{tid < U32.v nthr} -> slprop))
+  (#post : (tid:nat{tid < U32.v nthr} -> slprop))
+  (k :
+    (etid:erased nat{etid < U32.v nthr}) ->
+    stt unit (gpu ** thread_id etid ** pre etid)
+             (fun _ -> gpu ** thread_id etid ** post etid)
   )
-  : stt unit (cpu ** bigstar #u1 0 nthr pre)
-             (fun _ -> cpu ** bigstar #u1 0 nthr post)
+  requires cpu ** bigstar #u1 0 (U32.v nthr) pre
+  ensures  cpu ** bigstar #u1 0 (U32.v nthr) post
+```
