src/examples/matmul/GPU.MatMul.Pure.fsti
@@ -8,10 +8,10 @@ module U64 = FStar.UInt64
 
 let rec matmul_single
   (rows shared columns: nat)
-  (s1: erased (Seq.Base.seq U64.t){ Seq.Base.length s1 == rows * shared })
-  (s2 : erased (Seq.Base.seq U64.t){ Seq.Base.length s2 == shared * columns })
-  (row: erased nat{row < rows}) (col: erased nat{col < columns}) (to: nat)
-    : GTot (erased U64.t) (decreases to)
+  (s1: (Seq.Base.seq U64.t){ Seq.Base.length s1 == rows * shared })
+  (s2 : (Seq.Base.seq U64.t){ Seq.Base.length s2 == shared * columns })
+  (row: nat{row < rows}) (col: nat{col < columns}) (to: nat)
+    : GTot U64.t (decreases to)
   =
   if reveal to > shared then 0UL else if reveal to = 0 then 0UL else
     (
@@ -19,12 +19,12 @@ let rec matmul_single
         U64.add_mod (U64.mul_mod (Seq.Base.index s1 (row * shared + (to - 1))) (Seq.Base.index s2 (col + (to - 1) * columns))) (matmul_single rows shared columns s1 s2 row col (to - 1))
     )
 
-#push-options "--retry 2"
+#push-options "--retry 2" 
 let matmul_single_lemma
-  (rows shared columns: erased nat)
-  (s1: erased (Seq.Base.seq U64.t){ Seq.Base.length s1 == rows * shared })
-  (s2 : erased (Seq.Base.seq U64.t){ Seq.Base.length s2 == shared * columns })
-  (row: erased nat{row < rows}) (col: erased nat{col < columns}) (to: nat)
+  (rows shared columns: nat)
+  (s1: Seq.Base.seq U64.t{ Seq.Base.length s1 == rows * shared })
+  (s2 : Seq.Base.seq U64.t{ Seq.Base.length s2 == shared * columns })
+  (row: nat{row < rows}) (col: nat{col < columns}) (to: nat)
     : Lemma
       (requires (0 < to /\ to <= shared))
       (ensures (
@@ -35,26 +35,26 @@ let matmul_single_lemma
 #pop-options
 
 private let matmul_single_at
-  (rows shared columns: erased nat)
-  (s1: erased (Seq.Base.seq U64.t){ Seq.Base.length s1 == rows * shared })
-  (s2 : erased (Seq.Base.seq U64.t){ Seq.Base.length s2 == shared * columns })
+  (rows shared columns: nat)
+  (s1: (Seq.Base.seq U64.t){ Seq.Base.length s1 == rows * shared })
+  (s2 : (Seq.Base.seq U64.t){ Seq.Base.length s2 == shared * columns })
   (idx: nat{idx < rows * columns})
     : GTot U64.t
   =
   let row = idx / columns in let col = idx % columns in matmul_single rows shared columns s1 s2 row col shared
 
 let matmul
-  (rows shared columns: erased nat)
-  (s1: erased (Seq.Base.seq U64.t){ Seq.Base.length s1 == rows * shared })
-  (s2 : erased (Seq.Base.seq U64.t){ Seq.Base.length s2 == shared * columns })
+  (rows shared columns: nat)
+  (s1: (Seq.Base.seq U64.t){ Seq.Base.length s1 == rows * shared })
+  (s2 : (Seq.Base.seq U64.t){ Seq.Base.length s2 == shared * columns })
     : GTot (sr:(Seq.Base.seq U64.t){ Seq.Base.length sr == rows * columns })
   =
   Seq.Base.init_ghost (rows * columns) (matmul_single_at rows shared columns s1 s2)
 
 let lemma_matmul_index
-  (rows shared columns: erased nat)
-  (s1: erased (Seq.Base.seq U64.t){ Seq.Base.length s1 == rows * shared })
-  (s2 : erased (Seq.Base.seq U64.t){ Seq.Base.length s2 == shared * columns })
+  (rows shared columns: nat)
+  (s1: (Seq.Base.seq U64.t){ Seq.Base.length s1 == rows * shared })
+  (s2 : (Seq.Base.seq U64.t){ Seq.Base.length s2 == shared * columns })
   (idx: nat{idx < rows * columns})
     : Lemma
       (ensures (Seq.Base.index (reveal (matmul rows shared columns s1 s2)) idx) == reveal (matmul_single rows shared columns s1 s2 (idx / columns) (idx % columns) shared))
