src/lib/GPU.SizeT.fsti
@@ -1,0 +1,30 @@
+module GPU.SizeT
+
+open FStar.Ghost
+module SZ = FStar.SizeT
+module U32 = FStar.UInt32
+module U64 = FStar.UInt64
+
+(* Throughout this repo we assume a 64bit machine. This
+simplifies reasoning about overflow a bit. *)
+assume SizeTFitsU64 : FStar.SizeT.fits_u64
+assume SizeTFitsU32 : FStar.SizeT.fits_u32
+
+let fits_sizet (x:nat)
+  : Lemma (requires x < 0x10000000000000000)
+          (ensures FStar.SizeT.fits x)
+          [SMTPat (FStar.SizeT.fits x)]
+  = assert_norm (pow2 64 == 0x10000000000000000);
+    FStar.SizeT.fits_u64_implies_fits x
+
+[@@coercion] unfold let sizet_to_int  (x: SZ.t)  : GTot int = SZ.v x
+[@@coercion] unfold let u32_to_int    (x: U32.t) : GTot int = U32.v x
+[@@coercion] unfold let u64_to_int    (x: U64.t) : GTot int = U64.v x
+[@@coercion] unfold let sizet_to_eint (x: SZ.t)  : erased int = SZ.v x
+[@@coercion] unfold let u32_to_eint   (x: U32.t) : erased int = U32.v x
+[@@coercion] unfold let u64_to_eint   (x: U64.t) : erased int = U64.v x
+
+(* assumption, add to F*? *)
+val sizet_to_u32 (x: SZ.t) 
+  : Pure U32.t (requires FStar.UInt.fits (SZ.v x) 32)
+               (ensures fun r -> U32.v r == SZ.v x)
