src/lib/GPU.fsti
@@ -3,3 +3,4 @@ module GPU
 include GPU.Base
 include GPU.Ref
 include GPU.Array
+include GPU.SizeT
