test.sh
@@ -1,0 +1,30 @@
+#!/bin/bash
+
+set -eux
+
+MOD=GPU.DotProduct
+
+FILE=${MOD}.fst
+OFILE=GPU_DotProduct.c
+
+make -j32 -f Makefile.verify .cache/${FILE}.checked
+
+V=1 ./pulse.sh src/examples/${FILE} --codegen krml --extract GPU.Ref,GPU.Array,GPU.Base,${MOD} --debug extraction
+
+/home/guido/r/karamel/krml \
+	-add-early-include '"../GPU.h"' \
+	-fc++-compat \
+	-fcast-allocations \
+	-verbose -dast \
+	-skip-compilation -warn-error -2 -tmpdir kout \
+	.out/out.krml
+
+# Stuff to add to karamel:
+
+# Somehow the kcall has an extra unit(?) arg
+# sed -i 's/PULSE_KCALL\(.*\), (void \*)0U/PULSE_KCALL\1/' kout/"${OFILE}"
+
+# File extension
+ln -sf "${OFILE}" kout/final.cu
+
+nvcc -c kout/final.cu -o kout/final.o -I /home/guido/r/karamel/include/ -I /home/guido/r/karamel/krmllib/dist/minimal/
